stdlib/lampe/Stdlib/Collections/Map.lean
@@ -1,6 +1,0 @@
-import «std-1.0.0-beta.14».Extracted
-import Lampe
-
-namespace Lampe.Stdlib.Collections.Map
-
-open «std-1.0.0-beta.14»
