stdlib/lampe/std-1.0.0-beta.25.lean
@@ -1,0 +1,3 @@
+
+import «std-1.0.0-beta.25».Extracted
+
